Prove findCellAndMoveForward

formal-proofs/theories/lib/concurrent_linked_list/infinite_array/array_impl.v
@@ -1,6 +1,7 @@
 From iris.heap_lang Require Export proofmode notation lang.
 Require Import SegmentQueue.lib.concurrent_linked_list.list_interfaces.
-Require Import SegmentQueue.lib.concurrent_linked_list.infinite_array.sqsegment_impl.
+From SegmentQueue.lib.concurrent_linked_list.infinite_array Require Import
+     array_interfaces sqsegment_impl.
 
 Section array_impl.
 
@@ -8,44 +9,40 @@ Variable (segment_size pointer_shift: positive).
 
 Variable list_impl: listInterface.
 
-Definition newInfiniteArray: val :=
-  newList list_impl.
-
-Definition cancelCell: val :=
-  λ: "ptr", onSlotCleaned list_impl (Fst "ptr").
-
 Definition fromSome: val :=
   λ: "this", match: "this" with
                InjL "v" => "undefined"
              | InjR "v" => "v"
              end.
 
-Definition findCell: val :=
-  λ: "ptr" "id",
-  let: "sid" := "id" `quot` #(Pos.to_nat segment_size) in
-  let: "cid" := "id" `rem` #(Pos.to_nat segment_size) in
-  let: "seg" := fromSome (findSegment list_impl "ptr" "sid") in
-  if: getId "seg" = "sid"
-  then ("seg", "cid")
-  else ("seg", #0).
+Definition getIdImpl := getId (SQSegment segment_size pointer_shift).
 
-Definition derefCellPointer: val :=
-  λ: "ptr", let: "seg" := Fst "ptr" in
-            let: "ix" := Snd "ptr" in
-            getDataLoc "seg" +ₗ "ix".
-
-Definition cellPointerId: val :=
-  λ: "ptr", let: "seg" := Fst "ptr" in
-            let: "ix" := Snd "ptr" in
-            getId "seg" * #(Pos.to_nat segment_size) + "ix".
-
-Definition cellPointerCleanPrev: val :=
-  λ: "ptr", cleanPrev list_impl (Fst "ptr").
-
-Definition cutoffMoveForward: val :=
-  λ: "cutoff" "ptr", moveForward list_impl "cutoff" (Fst "ptr").
-
-Definition cutoffGetPointer: val :=
-  λ: "cutoff", !"cutoff".
+Definition InfiniteArray :=
+  {| array_interfaces.cancelCell :=
+       λ: "ptr", onSlotCleaned list_impl (Fst "ptr");
+     array_interfaces.newInfiniteArray := newList list_impl;
+     array_interfaces.findCell :=
+       λ: "ptr" "id",
+       let: "sid" := "id" `quot` #(Pos.to_nat segment_size) in
+       let: "cid" := "id" `rem` #(Pos.to_nat segment_size) in
+       let: "seg" := fromSome (findSegment list_impl "ptr" "sid") in
+       if: getIdImpl "seg" = "sid"
+       then ("seg", "cid")
+       else ("seg", #0);
+     array_interfaces.derefCellPointer :=
+       λ: "ptr", let: "seg" := Fst "ptr" in
+                 let: "ix" := Snd "ptr" in
+                 getDataLoc "seg" +ₗ "ix";
+     array_interfaces.cutoffMoveForward :=
+       λ: "cutoff" "ptr", moveForward list_impl "cutoff" (Fst "ptr");
+     array_interfaces.cutoffGetPointer := λ: "cutoff", !"cutoff";
+     array_interfaces.cellPointerId :=
+       λ: "ptr", let: "seg" := Fst "ptr" in
+                 let: "ix" := Snd "ptr" in
+                 getIdImpl "seg"
+                 * #(Pos.to_nat segment_size) + "ix";
+     array_interfaces.cellPointerCleanPrev :=
+       λ: "ptr", cleanPrev list_impl (Fst "ptr");
+  |}.
 
 End array_impl.
