formal-proofs/theories/lib/concurrent_linked_list/infinite_array/array_helpers.v
@@ -1,0 +1,54 @@
+From iris.program_logic Require Import atomic.
+From iris.heap_lang Require Export proofmode notation lang.
+Require Export SegmentQueue.lib.concurrent_linked_list.infinite_array.array_spec.
+
+Section impl.
+
+Variable (array_interface: infiniteArrayInterface).
+
+Definition findCellAndMoveForward: val :=
+  λ: "ptr" "id" "startFrom",
+  (rec: "loop" <> := let: "cell" := findCell array_interface "startFrom" "id" in
+                    if: cutoffMoveForward array_interface "ptr" "cell"
+                    then "cell"
+                    else "loop" #()) #().
+
+End impl.
+
+Section proof.
+
+Context `{!heapG Σ}.
+
+Variable (array_interface: infiniteArrayInterface).
+Variable (array_spec: infiniteArraySpec Σ array_interface).
+
+Theorem findCellAndMoveForward_spec N γ co p (v: val) (source_id id: nat):
+  is_infinite_array _ _ array_spec N γ co -∗
+  is_infinite_array_cutoff_reading _ _ _ N γ p source_id -∗
+  <<< ∀ start_index, ▷ is_infinite_array_cutoff _ _ _ N γ v start_index >>>
+      findCellAndMoveForward array_interface v #id p @ ⊤ ∖ ↑N
+  <<< ∃ p' id', is_infinite_array_cell_pointer _ _ _ N γ p' id'
+                ∗ ⌜(id ≤ id')%nat⌝
+                ∗ (∀ i, (⌜max source_id id ≤ i < id'⌝)%nat
+                        -∗ cell_is_cancelled _ _ _ N γ i)
+                ∗ ∃ i', ⌜start_index ≤ i' ≤ max id' start_index⌝ ∧
+                  is_infinite_array_cutoff _ _ _ N γ v i',
+  RET p' >>>.
+Proof.
+  iIntros "#HArr #HReading" (Φ) "AU". wp_lam. wp_pures. iLöb as "IH".
+  wp_bind (findCell _ _ _). iApply (findCell_spec with "[$]").
+  iIntros (p' id') "!> (#HCellPointer & % & #HCancelled)". wp_pures.
+  wp_bind (cutoffMoveForward _ _ _).
+  awp_apply (cutoffMoveForward_spec with "HArr HCellPointer").
+  iApply (aacc_aupd with "AU"); first done.
+  iIntros (start_index) "HCutoff". iAaccIntro with "HCutoff".
+  by iIntros "$ !> $ !> //".
+  iIntros ([|]) "HResult".
+  - iRight. iExists p', id'.
+    iSplitL; last by iIntros "!> HΦ !>"; wp_pures.
+    by iFrame "HCellPointer HCancelled HResult".
+  - iLeft. iFrame "HResult". iIntros "!> AU !>". wp_pures.
+    by iApply ("IH" with "AU").
+Qed.
+
+End proof.
