formal-proofs/theories/lib/concurrent_linked_list/infinite_array/array_interfaces.v
@@ -1,0 +1,13 @@
+From iris.heap_lang Require Export notation.
+
+Record infiniteArrayInterface :=
+  InfiniteArrayInterface {
+      newInfiniteArray: val;
+      cancelCell: val;
+      findCell: val;
+      derefCellPointer: val;
+      cutoffMoveForward: val;
+      cutoffGetPointer: val;
+      cellPointerId: val;
+      cellPointerCleanPrev: val;
+    }.
